mc_reify/nth_reif.v
@@ -1,0 +1,212 @@
+Require Import  Coq.Numbers.BinNums.
+Require Import compcert.lib.Maps.
+Require Import mc_reify.func_defs.
+
+Definition as_list (e : expr typ func) : option
+  ((typ * expr typ func * expr typ func) + typ) := 
+match e with
+  | Inj (inr (Data (fnil ty))) => Some (inr ty)
+  | App (App (Inj (inr (Data (fcons ty)))) hd) tl => Some (inl (ty, hd, tl))
+  | _ => None
+end.
+
+Fixpoint rnth_error (t: typ) (xs: expr typ func) (n: nat) : expr typ func :=
+  match as_list xs with
+  | Some (inr ty) => none_reif ty
+  | Some (inl (ty, hd, tl)) =>
+    match n with
+    | O => some_reif hd ty
+    | S n0 => rnth_error ty tl n0
+    end
+  | _ => App (Inj (inr (Data (fnth_error t n)))) xs
+  end.
+
+Fixpoint rreplace_nth (t: typ) (n: nat) (xs: expr typ func) (x: expr typ func) : expr typ func :=
+  match as_list xs with
+  | Some (inr ty) => xs
+  | Some (inl (ty, hd, tl)) => 
+    match n with
+    | O => App (App (Inj (inr (Data (fcons ty)))) x) tl
+    | S n0 => App (App (Inj (inr (Data (fcons ty)))) hd) (rreplace_nth t n0 tl x)
+    end
+  | _ => App (App (Inj (inr (Data (freplace_nth t n)))) xs) x
+  end.
+
+Require Import ExtLib.Tactics.
+Require Import solve_exprD.
+
+Section tbled.
+
+Variable tbl : SymEnv.functions RType_typ.
+
+Let RSym_sym := RSym_sym tbl.
+Existing Instance RSym_sym.
+
+Let RSym_sym_ok :  RSymOk RSym_sym := _.
+Existing Instance RSym_sym_ok.
+
+
+Let Expr_expr_fs := Expr_expr_fs tbl.
+Existing Instance Expr_expr_fs.
+
+Let Expr_ok_fs := Expr_ok_fs tbl.
+Existing Instance Expr_ok_fs.
+
+Existing Instance MA.
+
+Definition reflect tus tvs e (ty : typ)
+ := @exprD _ _ _ Expr_expr_fs tus tvs e ty.
+
+Lemma some_none: forall T v, @None T = Some v -> False. 
+intros. congruence.
+Qed.
+
+Lemma as_list_cons : forall e t hd tl,
+  as_list e = Some (inl (t, hd, tl)) ->
+  e = App (App (Inj (inr (Data (fcons t)))) hd) tl.
+Proof.
+  intros.
+  unfold as_list in H.
+  repeat
+  match goal with 
+  | [ H : match ?x with _ => _  end = _ |- _ ] => destruct x; 
+    try (apply some_none in H; contradiction) end.
+  congruence.
+  inversion H. subst. auto.
+Qed.
+
+Lemma as_list_nil : forall e t,
+  as_list e = Some (inr t) ->
+  e = Inj (inr (Data (fnil t))).
+Proof.
+  intros.
+  unfold as_list in H.
+  repeat
+  match goal with 
+  | [ H : match ?x with _ => _  end = _ |- _ ] => destruct x; 
+    try (apply some_none in H; contradiction) end.
+  inversion H. subst. auto.
+  congruence.
+Qed.
+
+Ltac solve_exprD := solve_exprD.solve_exprD tbl.
+
+Opaque type_cast.
+
+Ltac destruct_as_list :=
+repeat
+match goal with
+| [ H : context [ match as_list ?x with _ => _ end] |- _] => destruct (as_list x) eqn:? 
+| [ |- context [ match as_list ?x with _ => _ end]] => destruct (as_list x) eqn:? 
+| [ H : as_list _ = Some (inr _) |- _ ] => apply as_list_nil in H
+| [ H : as_list _ = Some (inl (_ , _, _)) |- _ ] => apply as_list_cons in H
+| [ H : as_list _ = Some (inl (?p, _)) |- _ ] => destruct p
+| [ H : as_list _ = Some (inl ?p) |- _ ] => destruct p
+| [ H : as_list _ = Some ?p |- _ ] => destruct p
+end;
+subst.
+
+Lemma rnth_error_eq2 :
+forall typ xs n tus tvs val,
+exprD' tus tvs (tylist typ) xs = Some val ->
+exprD' tus tvs (tyoption typ) (App (Inj (inr (Data (fnth_error typ n)))) xs)  =
+exprD' tus tvs (tyoption typ) (rnth_error typ xs n).
+Proof.
+intros.
+match goal with 
+        [ |- ?l = ?r ] => destruct l eqn:?, r eqn:?
+    end; auto.
+  + solve_exprD. simpl in *. unfold exprT_App. simpl. rewrite <- Heqo0.
+    clear Heqo0 e0.
+    generalize dependent e2.
+    generalize dependent xs.
+    induction n; intros.
+      - simpl in *. unfold some_reif, none_reif in *.
+        destruct_as_list; solve_exprD.
+      - simpl in *. unfold some_reif, none_reif in *.
+        destruct_as_list; solve_exprD.
+  + solve_exprD.
+    unfold exprT_App; simpl.
+    generalize dependent e1.
+    generalize dependent xs.
+    induction n; intros.
+      - simpl in *. unfold some_reif, none_reif in *.
+        destruct_as_list; solve_exprD.
+      - simpl in *. unfold some_reif, none_reif in *.
+        destruct_as_list; solve_exprD.
+  + unfold RSym_sym in *. solve_exprD.
+Qed.
+
+Lemma typeof_rreplace_nth: forall t xs x n tus tvs,
+  typeof_expr tus tvs xs = Some (tylist t) ->
+  typeof_expr tus tvs x = Some t ->
+  typeof_expr tus tvs (rreplace_nth t n xs x) = Some (tylist t).
+Proof.
+  intros.
+  revert xs H.
+  induction n; intros.
+  + simpl.
+    destruct_as_list.
+    - simpl in H |- *.
+      progress_match; simpl.
+      unfold Rty in *; subst; simpl.
+      inv_some.
+      solve_exprD.
+    - auto.
+    - solve_exprD.
+  + simpl. destruct_as_list.
+    - simpl in H |- *.
+      progress_match; simpl.
+      unfold Rty in *; subst; simpl.
+      inv_some.
+      rewrite IHn by auto.
+      solve_exprD.
+    - auto.
+    - solve_exprD.
+Qed.
+
+Lemma rreplace_nth_eq2 :
+forall typ xs x n tus tvs val v,
+exprD' tus tvs (tylist typ) xs = Some val ->
+exprD' tus tvs typ x = Some v ->
+exprD' tus tvs (tylist typ) (App (App (Inj (inr (Data (freplace_nth typ n)))) xs) x)  =
+exprD' tus tvs (tylist typ) (rreplace_nth typ n xs x).
+Proof.
+  fold func in *; unfold RSym_sym in *.
+  intros.
+  match goal with 
+        [ |- ?l = ?r ] => destruct l eqn:?, r eqn:?
+    end; auto.
+  + solve_exprD. simpl in *. unfold exprT_App. simpl. rewrite <- Heqo0.
+    clear Heqo0 e0.
+    generalize dependent e2.
+    generalize dependent xs.
+    induction n; intros.
+      - simpl in *. unfold some_reif, none_reif in *.
+        destruct_as_list; solve_exprD.
+      - simpl in *. unfold some_reif, none_reif in *.
+        destruct_as_list; solve_exprD.
+        simpl in H0.
+        progress_match.
+        solve_exprD.
+        unfold Rty in r; subst.
+        solve_exprD.
+        unfold exprT_App; simpl.
+        erewrite <- IHn with (e2 := e3); eauto.
+  + solve_exprD.
+    unfold exprT_App; simpl.
+    generalize dependent e1.
+    generalize dependent xs.
+    induction n; intros.
+      - simpl in *. unfold some_reif, none_reif in *.
+        destruct_as_list; solve_exprD.
+      - simpl in *. unfold some_reif, none_reif in *.
+        destruct_as_list; solve_exprD.
+        rewrite typeof_rreplace_nth in Heqo0 by auto.
+        solve_exprD.
+        specialize (IHn e Heqo4 Heqo2 _ Heqo5).
+        inversion IHn.
+  + unfold RSym_sym in *. solve_exprD.
+Qed.
+
+End tbled.
