mc_reify/solve_efield_denote.v
@@ -1,0 +1,123 @@
+Require Import floyd.proofauto.
+Require Import mc_reify.bool_funcs.
+Require Import Coq.Logic.JMeq.
+Local Open Scope logic.
+
+Require Export mc_reify.reify.
+Require Import mc_reify.set_reif.
+Require Import MirrorCore.Lemma.
+Require Import MirrorCharge.RTac.ReifyLemma.
+Require Import mc_reify.update_tycon.
+Require Export MirrorCore.RTac.Repeat.
+Require Import MirrorCore.RTac.Then.
+Require Export MirrorCore.RTac.Try.
+Require Export MirrorCore.RTac.First.
+Require Import MirrorCore.RTac.Fail.
+Require Import MirrorCore.RTac.Simplify.
+Require Import MirrorCore.Lambda.RedAll.
+Require Import MirrorCore.Lambda.ExprUnify_simul.
+Require Import MirrorCore.RTac.RTac.
+Require Import MirrorCharge.RTac.Instantiate.
+Require Import MirrorCharge.RTac.Intro.
+Require Import MirrorCharge.RTac.Apply.
+Require Import MirrorCharge.RTac.EApply.
+Require Export mc_reify.funcs.
+Require Import mc_reify.types.
+Require Export mc_reify.reflexivity_tacs.
+Require Import mc_reify.get_set_reif.
+Require Import mc_reify.func_defs.
+Require Import mc_reify.typ_eq.
+Require Import mc_reify.rtac_base.
+
+Lemma msubst_efield_denote_nil: forall T1 T2, msubst_efield_denote T1 T2 nil = Some nil.
+Proof.
+  intros.
+  reflexivity.
+Qed.
+
+Lemma msubst_efield_denote_cons_struct: forall fld efs T1 T2 gfs,
+  msubst_efield_denote T1 T2 efs = Some gfs ->
+  msubst_efield_denote T1 T2 (eStructField fld :: efs) = Some (StructField fld :: gfs).
+Proof.
+  intros.
+  simpl.
+  rewrite H.
+  reflexivity.
+Qed.
+
+Lemma msubst_efield_denote_cons_union: forall fld efs T1 T2 gfs,
+  msubst_efield_denote T1 T2 efs = Some gfs ->
+  msubst_efield_denote T1 T2 (eUnionField fld :: efs) = Some (UnionField fld :: gfs).
+Proof.
+  intros.
+  simpl.
+  rewrite H.
+  reflexivity.
+Qed.
+
+Lemma msubst_efield_denote_cons_array: forall ei efs T1 T2 i gfs,
+  msubst_efield_denote T1 T2 efs = Some gfs ->
+  type_is_int ei = true -> 
+  msubst_eval_LR T1 T2 ei RRRR = Some (Values.Vint i) ->
+  msubst_efield_denote T1 T2 (eArraySubsc ei :: efs) = Some (ArraySubsc (Int.unsigned i) :: gfs).
+Proof.
+  intros.
+  simpl.
+  unfold type_is_int in H0.
+  destruct (typeof ei); try inversion H0.
+  unfold msubst_eval_LR in H1.
+  rewrite H, H1.
+  reflexivity.
+Qed.
+
+(************************************************
+
+Reified Lemmas
+
+************************************************)
+
+Definition msubst_efield_denote_nil_lemma: my_lemma.
+reify_lemma reify_vst msubst_efield_denote_nil.
+Defined.
+
+(* Print msubst_efield_denote_nil_lemma. *)
+
+Definition msubst_efield_denote_cons_struct_lemma (fld: ident) (efs: list efield) : my_lemma.
+reify_lemma reify_vst (msubst_efield_denote_cons_struct fld efs).
+Defined.
+
+Definition msubst_efield_denote_cons_union_lemma (fld: ident) (efs: list efield) : my_lemma.
+reify_lemma reify_vst (msubst_efield_denote_cons_union fld efs).
+Defined.
+
+Definition msubst_efield_denote_cons_array_lemma (ei: Clight.expr) (efs: list efield) : my_lemma.
+reify_lemma reify_vst (msubst_efield_denote_cons_array ei efs).
+Defined.
+
+(* Print msubst_efield_denote_cons_array_lemma. *)
+
+Section tbled.
+
+Variable tbl : SymEnv.functions RType_typ.
+Let RSym_sym := RSym_sym tbl.
+Existing Instance RSym_sym.
+
+Fixpoint solve_efield_denote (efs: list efield) : rtac typ (expr typ func) :=
+  match efs with
+  | nil => EAPPLY typ func msubst_efield_denote_nil_lemma
+  | eStructField fld :: efs0 => 
+      THEN (EAPPLY typ func (msubst_efield_denote_cons_struct_lemma fld efs0))
+        (solve_efield_denote efs0)
+  | eUnionField fld :: efs0 => 
+      THEN (EAPPLY typ func (msubst_efield_denote_cons_union_lemma fld efs0))
+        (solve_efield_denote efs0)
+  | eArraySubsc ei :: efs0 => 
+      THEN (THEN (EAPPLY typ func (msubst_efield_denote_cons_array_lemma ei efs0))
+        (TRY (REFLEXIVITY_MSUBST tbl)))
+        (solve_efield_denote efs0)
+  end.
+
+
+Check data_at.
+Check Vfloat.
+SearchAbout float.
