mc_reify/verif_nest3_bm.v
@@ -1,0 +1,474 @@
+Require Import floyd.proofauto.
+Require Import progs.nest3.
+
+Local Open Scope logic.
+
+Definition get_spec :=
+ DECLARE _get
+  WITH v : reptype' t_struct_c, p: val
+  PRE  [] 
+        PROP  ()
+        LOCAL (var _p t_struct_c p)
+        SEP   (`(data_at Ews t_struct_c (repinj _ v) p))
+  POST [ tint ]
+        PROP  ()
+        LOCAL (var _p t_struct_c p; temp 1%positive (Vint (snd (snd (snd v)))))
+        SEP   (`(data_at Ews t_struct_c (repinj _ v) p)).
+
+Definition update222 (i: int) (v: reptype' t_struct_c) : reptype' t_struct_c :=
+   (fst v, (fst (snd v), (fst (snd (snd v)), i))).
+
+Definition set_spec :=
+ DECLARE _set
+  WITH i : int, v : reptype' t_struct_c, p : val
+  PRE  [ _i OF tint ] 
+        PROP ()
+        LOCAL(temp _i (Vint i); var _p t_struct_c p)
+        SEP(`(data_at Ews t_struct_c (repinj _ v) p))
+  POST [ tvoid ]
+        `(data_at Ews t_struct_c (repinj _ (update222 i v)) p).
+
+Definition multi_command_spec :=
+ DECLARE _multi_command
+  WITH i111: int,
+       i112: int,
+       i121: int,
+       i122: int,
+       i211: int,
+       i212: int,
+       i221: int,
+       i222: int,
+       p: val
+  PRE  []
+        PROP ()
+        LOCAL(var _p t_struct_c p)
+        SEP(`(data_at Ews t_struct_c
+               (repinj t_struct_c (((i111, i112), (i121, i122)), ((i211, i212), (i221, i222)))) p))
+  POST [ tvoid ]
+            `(data_at Ews t_struct_c
+               (repinj t_struct_c (((i111, i112), (i121, i122)),
+                          ((Int.add i122 (Int.repr 4), Int.add i121 (Int.repr 3)),
+                           (Int.add i112 (Int.repr 2), Int.add i111 (Int.repr 1))))) p).
+
+Definition multi_command_spec' :=
+ DECLARE _multi_command
+  WITH i111: int,
+       i112: int,
+       i121: int,
+       i122: int,
+       i211: int,
+       i212: int,
+       i221: int,
+       i222: int,
+       p: val,
+       q: val
+  PRE  []
+        PROP ()
+        LOCAL(var _p t_struct_c p)
+        SEP(`(data_at Ews t_struct_c (default_val _) q);
+            `(data_at Ews t_struct_c
+               (repinj t_struct_c (((i111, i112), (i121, i122)), ((i211, i212), (i221, i222)))) p))
+  POST [ tvoid ]
+            `(data_at Ews t_struct_c (default_val _) q) * 
+            `(data_at Ews t_struct_c
+               (repinj t_struct_c (((i111, i112), (i121, i122)),
+                          ((Int.add i122 (Int.repr 4), Int.add i121 (Int.repr 3)),
+                           (Int.add i112 (Int.repr 2), Int.add i111 (Int.repr 1))))) p).
+
+Definition multi_command_s_spec :=
+ DECLARE _multi_command_s
+  WITH p0: val,
+       p1: val,
+       p2: val,
+       p3: val,
+       p4: val,
+       p5: val,
+       p6: val,
+       p7: val
+  PRE  []
+        PROP ()
+        LOCAL(var _p0 tint p0;
+              var _p1 tint p1;
+              var _p2 tint p2;
+              var _p3 tint p3;
+              var _p4 tint p4;
+              var _p5 tint p5;
+              var _p6 tint p6;
+              var _p7 tint p7)
+        SEP(`(data_at Ews tint (Vint (Int.repr 0)) p0);
+            `(data_at Ews tint (Vint (Int.repr 0)) p1);
+            `(data_at Ews tint (Vint (Int.repr 0)) p2);
+            `(data_at Ews tint (Vint (Int.repr 0)) p3);
+            `(data_at Ews tint (Vint (Int.repr 0)) p4);
+            `(data_at Ews tint (Vint (Int.repr 0)) p5);
+            `(data_at Ews tint (Vint (Int.repr 0)) p6);
+            `(data_at Ews tint (Vint (Int.repr 0)) p7))
+  POST [ tvoid ]
+        PROP ()
+        LOCAL(var _p0 tint p0;
+              var _p1 tint p1;
+              var _p2 tint p2;
+              var _p3 tint p3;
+              var _p4 tint p4;
+              var _p5 tint p5;
+              var _p6 tint p6;
+              var _p7 tint p7)
+        SEP(`(data_at Ews tint (Vint (Int.repr 0)) p0);
+            `(data_at Ews tint (Vint (Int.repr 0)) p1);
+            `(data_at Ews tint (Vint (Int.repr 0)) p2);
+            `(data_at Ews tint (Vint (Int.repr 0)) p3);
+            `(data_at Ews tint (Vint (Int.repr 4)) p4);
+            `(data_at Ews tint (Vint (Int.repr 3)) p5);
+            `(data_at Ews tint (Vint (Int.repr 2)) p6);
+            `(data_at Ews tint (Vint (Int.repr 1)) p7)).
+
+Definition Vprog : varspecs := (_p, t_struct_c)::
+                               (_p0, tint)::
+                               (_p1, tint)::
+                               (_p2, tint)::
+                               (_p3, tint)::
+                               (_p4, tint)::
+                               (_p5, tint)::
+                               (_p6, tint)::
+                               (_p7, tint)::
+                               nil.
+
+Definition Gprog : funspecs := 
+    multi_command_s_spec::multi_command_spec::nil.
+
+Require Import Timing.
+(*
+Ltac lforward :=
+start_timer "Forward";
+forward.forward;
+stop_timer "Forward".
+
+Clear Timing Profile.
+
+Lemma body_multi_command: semax_body Vprog Gprog f_multi_command multi_command_spec.
+Proof.
+  start_function.
+start_timer "T08a Folded Ltac".
+  lforward; [entailer! | solve_legal_nested_field_in_entailment' |].
+  lforward; [entailer! | solve_legal_nested_field_in_entailment' x|].
+  simpl upd_reptype.
+  lforward; [entailer! | solve_legal_nested_field_in_entailment' |].
+  lforward; [entailer! | solve_legal_nested_field_in_entailment' |].
+  simpl upd_reptype.
+  lforward; [entailer! | solve_legal_nested_field_in_entailment' |].
+  lforward; [entailer! | solve_legal_nested_field_in_entailment' |].
+  simpl upd_reptype.
+  lforward; [entailer! | solve_legal_nested_field_in_entailment' |].
+  lforward; [entailer! | solve_legal_nested_field_in_entailment' |].
+  simpl upd_reptype.
+stop_timer "T08a Folded Ltac".
+  forward.forward. (* return *)
+Qed.
+
+Print Timing Profile.
+*)
+
+(*
+Lemma body_multi_command2: semax_body Vprog Gprog f_multi_command multi_command_spec.
+Proof.
+  start_function.
+  unfold_data_at 1%nat.
+  unfold_field_at 1%nat.
+  unfold_field_at 3%nat.
+  unfold_field_at 1%nat.
+  unfold_field_at 3%nat.
+  unfold_field_at 5%nat.
+  unfold_field_at 7%nat.
+start_timer "T08a Unfolded Ltac".
+  forward.forward; [entailer! | solve_legal_nested_field_in_entailment' |].
+  forward.forward; [entailer! | solve_legal_nested_field_in_entailment' |].
+  simpl upd_reptype.
+  forward.forward; [entailer! | solve_legal_nested_field_in_entailment' |].
+  forward.forward; [entailer! | solve_legal_nested_field_in_entailment' |].
+  simpl upd_reptype.
+  forward.forward; [entailer! | solve_legal_nested_field_in_entailment' |].
+  forward.forward; [entailer! | solve_legal_nested_field_in_entailment' |].
+  simpl upd_reptype.
+  forward.forward; [entailer! | solve_legal_nested_field_in_entailment' |].
+  forward.forward; [entailer! | solve_legal_nested_field_in_entailment' |].
+  simpl upd_reptype.
+stop_timer "T08a Unfolded Ltac".
+  forward.forward. (* return *)
+  unfold_data_at 1%nat.
+  unfold_field_at 9%nat.
+  unfold_field_at 11%nat.
+  unfold_field_at 9%nat.
+  unfold_field_at 11%nat.
+  unfold_field_at 13%nat.
+  unfold_field_at 15%nat.
+  entailer!.
+Qed.
+
+Lemma body_multi_command3: semax_body Vprog Gprog f_multi_command multi_command_spec'.
+Proof.
+  start_function.
+  unfold_data_at 1%nat.
+  unfold_data_at 1%nat.
+  unfold_field_at 1%nat.
+  unfold_field_at 3%nat.
+  unfold_field_at 5%nat.
+  unfold_field_at 7%nat.
+  unfold_field_at 1%nat.
+  unfold_field_at 3%nat.
+  unfold_field_at 5%nat.
+  unfold_field_at 7%nat.
+  unfold_field_at 9%nat.
+  unfold_field_at 11%nat.
+  unfold_field_at 13%nat.
+  unfold_field_at 15%nat.
+start_timer "T16 Unfolded Ltac".
+  forward.forward; [entailer! | solve_legal_nested_field_in_entailment' |].
+  forward.forward; [entailer! | solve_legal_nested_field_in_entailment' |].
+  simpl upd_reptype.
+  forward.forward; [entailer! | solve_legal_nested_field_in_entailment' |].
+  forward.forward; [entailer! | solve_legal_nested_field_in_entailment' |].
+  simpl upd_reptype.
+  forward.forward; [entailer! | solve_legal_nested_field_in_entailment' |].
+  forward.forward; [entailer! | solve_legal_nested_field_in_entailment' |].
+  simpl upd_reptype.
+  forward.forward; [entailer! | solve_legal_nested_field_in_entailment' |].
+  forward.forward; [entailer! | solve_legal_nested_field_in_entailment' |].
+  simpl upd_reptype.
+stop_timer "T16 Unfolded Ltac".
+  forward.forward. (* return *)
+  unfold_data_at 1%nat.
+  unfold_data_at 1%nat.
+  unfold_field_at 17%nat.
+  unfold_field_at 19%nat.
+  unfold_field_at 21%nat.
+  unfold_field_at 23%nat.
+  unfold_field_at 17%nat.
+  unfold_field_at 19%nat.
+  unfold_field_at 21%nat.
+  unfold_field_at 23%nat.
+  unfold_field_at 25%nat.
+  unfold_field_at 27%nat.
+  unfold_field_at 29%nat.
+  unfold_field_at 31%nat.
+  cancel.
+Qed.
+*)
+(*
+Clear Timing Profile.
+Lemma body_multi_command_s: semax_body Vprog Gprog f_multi_command_s multi_command_s_spec.
+Proof.
+  start_function.
+start_timer "T08b Unfolded Ltac".
+  lforward; [entailer! | solve_legal_nested_field_in_entailment' |].
+  lforward; [entailer! | solve_legal_nested_field_in_entailment' |].
+  simpl upd_reptype.
+  lforward; [entailer! | solve_legal_nested_field_in_entailment' |].
+  lforward; [entailer! | solve_legal_nested_field_in_entailment' |].
+  simpl upd_reptype.
+  lforward; [entailer! | solve_legal_nested_field_in_entailment' |].
+  lforward; [entailer! | solve_legal_nested_field_in_entailment' |].
+  simpl upd_reptype.
+  lforward; [entailer! | solve_legal_nested_field_in_entailment' |].
+  lforward; [entailer! | solve_legal_nested_field_in_entailment' |].
+  simpl upd_reptype.
+stop_timer "T08b Unfolded Ltac".
+  forward.forward. (* return *)
+  cancel.
+Qed.
+*)
+Print Timing Profile.
+
+Require Export mc_reify.symexe_soundness.
+
+Require Import MirrorCore.RTac.Repeat.
+Require Import MirrorCore.RTac.Then.
+Require Import MirrorCore.RTac.Try.
+Require Import MirrorCore.RTac.First.
+Require Import MirrorCore.RTac.Fail.
+Require Import MirrorCore.RTac.Simplify.
+Require Import MirrorCore.RTac.RTac.
+Require Import mc_reify.types.
+Require Import mc_reify.funcs.
+Require Import mc_reify.func_defs.
+Require Import mc_reify.app_lemmas.
+Require Import MirrorCore.LemmaApply.
+Require Import ExtLib.Tactics.
+Require Import MirrorCore.Util.ListMapT.
+Require Import MirrorCharge.RTac.Instantiate.
+Require Import MirrorCharge.RTac.Intro.
+Require Import MirrorCharge.RTac.Apply.
+Require Import MirrorCharge.RTac.EApply.
+Require Import mc_reify.rtac_base.
+Require Import mc_reify.reified_ltac_lemmas.
+Require Import mc_reify.hoist_later_in_pre.
+Require Import mc_reify.set_load_store.
+Require Import mc_reify.symexe.
+
+(*
+Lemma body_multi_command_s2: semax_body Vprog nil f_multi_command_s multi_command_s_spec.
+Proof.
+  start_function.
+
+start_timer "T08b Unfolded Rtac".
+
+unfold abbreviate in Delta, (*MORE_COMMANDS,*) POSTCONDITION.
+subst Delta (*MORE_COMMANDS*) POSTCONDITION.
+ensure_normal_ret_assert.
+match goal with
+| |- semax _ _ _ (normal_ret_assert ?M) => set (POSTCONDITION := M)
+end.
+
+prepare_reify.
+unfold PTree.set, PTree.prev, tarray, tint; simpl.
+
+rforward.
+
+repeat split.
++ intros.
+  apply andp_right.
+  entailer!.
+  apply prop_right. solve_legal_nested_field.
++ intros.
+  apply prop_right. solve_legal_nested_field.
++ intros.
+  apply andp_right.
+  entailer!.
+  apply prop_right. solve_legal_nested_field.
++ intros.
+  apply prop_right. solve_legal_nested_field.
++ intros.
+  apply andp_right.
+  entailer!.
+  apply prop_right. solve_legal_nested_field.
++ intros.
+  apply prop_right. solve_legal_nested_field.
++ intros.
+  apply andp_right.
+  entailer!.
+  apply prop_right. solve_legal_nested_field.
++ intros.
+  apply prop_right. solve_legal_nested_field.
++ 
+stop_timer "T08b Unfolded Rtac".
+admit.
+Qed.
+Print Timing Profile.
+*)
+Lemma body_multi_command4: semax_body Vprog nil f_multi_command multi_command_spec.
+Proof.
+  start_function.
+start_timer "T08a Folded Rtac".
+
+unfold abbreviate in Delta, MORE_COMMANDS, POSTCONDITION.
+subst Delta MORE_COMMANDS POSTCONDITION.
+ensure_normal_ret_assert.
+match goal with
+| |- semax _ _ _ (normal_ret_assert ?M) => set (POSTCONDITION := M)
+end.
+
+prepare_reify.
+unfold t_struct_c, t_struct_b, t_struct_a in *; simpl.
+unfold PTree.set, PTree.prev, tarray, tint; simpl.
+
+(*
+match goal with
+| |- semax ?Delta ?Pre (Ssequence (Ssequence ?A1 (Ssequence ?A2 (Ssequence ?A3 _))) _)  _ =>
+   assert (semax Delta Pre (Ssequence A1 Sskip)
+   (normal_ret_assert Pre)); [| admit]
+end.
+(*
+ 08 reduce:	(total:0.057167, mean:0.057167, runs:1, sigma2:0.000000)
+   09 cut1:	(total:0.118262, mean:0.118262, runs:1, sigma2:0.000000)
+ 10 change:	(total:0.000002, mean:0.000002, runs:1, sigma2:0.000000)
+   11 cut2:	(total:0.184445, mean:0.184445, runs:1, sigma2:0.000000)
+*)
+*)
+
+(*
+match goal with
+| |- semax ?Delta ?Pre (Ssequence (Ssequence ?A1 (Ssequence ?A2 (Ssequence ?A3 _))) _)  _ =>
+   assert (semax Delta Pre (Ssequence A1 (Ssequence A2 Sskip))
+   (normal_ret_assert Pre)); [| admit]
+end.
+(*
+ 08 reduce:	(total:0.079519, mean:0.079519, runs:1, sigma2:0.000000)
+   09 cut1:	(total:0.284411, mean:0.284411, runs:1, sigma2:0.000000)
+ 10 change:	(total:0.000001, mean:0.000001, runs:1, sigma2:0.000000)
+   11 cut2:	(total:0.307770, mean:0.307770, runs:1, sigma2:0.000000)
+*)
+*)
+
+(*
+match goal with
+| |- semax ?Delta ?Pre (Ssequence (Ssequence ?A1 (Ssequence ?A2 (Ssequence ?A3 _))) _)  _ =>
+   assert (semax Delta Pre (Ssequence A1 (Ssequence A2 (Ssequence A3 Sskip)))
+   (normal_ret_assert Pre)); [| admit]
+end.
+(*
+05 vm_compute:	(total:0.093451, mean:0.093451, runs:1, sigma2:0.000000)
+ 08 reduce:	(total:0.223416, mean:0.223416, runs:1, sigma2:0.000000)
+   09 cut1:	(total:1.312236, mean:1.312236, runs:1, sigma2:0.000000)
+ 10 change:	(total:0.000002, mean:0.000002, runs:1, sigma2:0.000000)
+   11 cut2:	(total:1.057662, mean:1.057662, runs:1, sigma2:0.000000)
+*)
+*)
+
+(*
+match goal with
+| |- semax ?Delta ?Pre (Ssequence (Ssequence ?A1 (Ssequence ?A2 (Ssequence ?A3 (Ssequence ?A4 _)))) _)  _ =>
+   assert (semax Delta Pre (Ssequence A1 (Ssequence A2 (Ssequence A3 (Ssequence A4 Sskip))))
+   (normal_ret_assert Pre)); [| admit]
+end.
+(*
+ 05 vm_compute:	(total:0.154376, mean:0.154376, runs:1, sigma2:0.000000)
+ 08 reduce:	(total:0.784162, mean:0.784162, runs:1, sigma2:0.000000)
+   09 cut1:	(total:6.706352, mean:6.706352, runs:1, sigma2:0.000000)
+ 10 change:	(total:0.000002, mean:0.000002, runs:1, sigma2:0.000000)
+   11 cut2:	(total:5.556991, mean:5.556991, runs:1, sigma2:0.000000)
+*)
+*)
+(*
+match goal with
+| |- semax ?Delta ?Pre (Ssequence (Ssequence ?A1 (Ssequence ?A2 (Ssequence ?A3 (Ssequence ?A4 
+         (Ssequence ?A5 (Ssequence ?A6 (Ssequence ?A7 ?A8))))))) _)  _ =>
+   assert (semax Delta Pre (Ssequence A1 (Ssequence A3 (Ssequence A5 (Ssequence A7 
+                             (Ssequence A1 (Ssequence A3 (Ssequence A5 (Ssequence A7 Sskip))))))))
+   (normal_ret_assert Pre)); [| admit]
+end.
+*)
+Set Printing Depth 4. 
+Clear Timing Profile.
+rforward.
+Print Timing Profile.
+
+repeat split.
++ Set Printing Depth 50. 
+  intros.
+  apply andp_right.
+  entailer!.
+  apply prop_right. solve_legal_nested_field.
++ intros.
+  apply prop_right. solve_legal_nested_field.
++ intros.
+  apply andp_right.
+  entailer!.
+  apply prop_right. solve_legal_nested_field.
++ intros.
+  apply prop_right. solve_legal_nested_field.
++ intros.
+  apply andp_right.
+  entailer!.
+  apply prop_right. solve_legal_nested_field.
++ intros.
+  apply prop_right. solve_legal_nested_field.
++ intros.
+  apply andp_right.
+  entailer!.
+  apply prop_right. solve_legal_nested_field.
++ intros.
+  apply prop_right. solve_legal_nested_field.
++ 
+stop_timer "T08a Folded Rtac".
+admit.
+
+Qed.
